\documentclass{article}
\usepackage{epsfig}
\pagestyle{empty}
\begin{document}
$1.60217738 \cdot 10^{-19} C$
\pagebreak

$9.1093897 \cdot 10^{-31}$
\pagebreak

$1.6726230 \cdot 10^{-27}$
\pagebreak

$1.6749286 \cdot 10^{-27}$
\pagebreak

$mol^{-1}$
\pagebreak

$6.0221367 \cdot 10^{23} mol^{-1}$
\pagebreak

$1.380657 \cdot 10^{-23}$
\pagebreak

$6.6260754 \cdot 10^{-34}$
\pagebreak

$5.29177249 \cdot 10^{-11}$
\pagebreak

$C^2J^{-1}m^{-1}$
\pagebreak

$8.85419 \cdot 10^{-12} C^2J^{-1}m^{-1}$
\pagebreak

$Js^2C^{-2}m^{-1}$
\pagebreak

$4\pi \cdot 10^{-7} Js^2C^{-2}m^{-1}$
\pagebreak

$2.99792458 \cdot 10^8 ms^{-1}$
\pagebreak

$Nm^2kg^{-2}$
\pagebreak

$6.67259 \cdot 10^{-11} Nm^2kg^{-2}$
\pagebreak

$7.29735 \cdot 10^{-3}$
\pagebreak

\[\mathrm \varepsilon = 4 r_{ij}\nonumber \]
\pagebreak

$ {\AA}/ps $
\pagebreak

$ \begin{array}{ccccccccc} a_{1,1} x_1 & + & a_{1,2} x_2 & + & \ldots & + & a_{1,n} x_n & = & a_{1,(n+1)} \\ a_{2,1} x_1 & + & a_{2,2} x_2 & + & \ldots & + & a_{2,n} x_n & = & a_{2,(n+1)} \\ \vdots & & \vdots & & \ddots & & \vdots & & \vdots \\ a_{n,1} x_1 & + & a_{n,2} x_2 & + & \ldots & + & a_{n,n} x_n & = & a_{n,(n+1)} \\ \end{array} $
\pagebreak

$x = (x_1, x_2,\ldots x_N)$
\pagebreak

$n\times(n+1)$
\pagebreak

$ a_{1,1}, a_{1,2}, \cdot, a_{1,(n+1)}, a_{2,1}, \ldots a_{n,(n+1)} $
\pagebreak

$a_1 x_1 + b_1 x_2 = c_1$
\pagebreak

$a_2 x_1 + b_2 x_2 = c_2$
\pagebreak

$x^2 + b x + c = 0$
\pagebreak

$0 \le \mathtt{angle} \le 360, 0 \le angle \le 2 \pi$
\pagebreak

$-180 \le \mathtt{angle} \le 180, -\pi \le \mathtt{angle} \le \pi$
\pagebreak

$\{x|y|z|\} *= \sqrt{x^2 + y^2 + z^2}$
\pagebreak

$var1=atan(.5); sin(cos(atan(asin(exp(X+var1)))))$
\pagebreak

$X$
\pagebreak

$p$
\pagebreak

\[\sum_{i=0}^{d} a_i^{(k)} (x - x_0^{(k)})^i\]
\pagebreak

$k$
\pagebreak

$d$
\pagebreak

$\{x|y|z\} *= \sqrt{x^2 + y^2 + z^2}$
\pagebreak

$\sqrt{x^2 + y^2}$
\pagebreak

$x^2 + y^2$
\pagebreak

$\{x|y|z\} *= \sqrt{x^2 + y^2}$
\pagebreak

$2 \pi$
\pagebreak

$\pi$
\pagebreak

\[ x = r \sin \theta \cos \phi \]
\pagebreak

\[ y = r \sin \theta \sin \phi \]
\pagebreak

\[ z = r \cos \theta \]
\pagebreak

$\sqrt{x^2 + y^2 + z^2}$
\pagebreak

$x^2 + y^2 + z^2$
\pagebreak

$\sqrt{x^2 + y^2 + z^2 + h^2}$
\pagebreak

$x^2 + y^2 + z^2 + h^2$
\pagebreak

$\{x|y|z|h\} *= \sqrt{x^2 + y^2 + z^2 + h^2}$
\pagebreak

${\AA}$
\pagebreak

$\geq 0$
\pagebreak

$g^T \cdot g$
\pagebreak

$g$
\pagebreak

$step\cdot|direction|$
\pagebreak

\[E_{k+1} \leq E_k + \alpha\cdot stp\cdot<g_k, d_k>\]
\pagebreak

\[|<g_{k+1}, d_k>| \leq \beta\cdot |<g_k, d_k>|\]
\pagebreak

$g_k$
\pagebreak

$g_{k+1}$
\pagebreak

$d_k$
\pagebreak

$E_{k+1}$
\pagebreak

$E_k$
\pagebreak

$\alpha$
\pagebreak

$\beta$
\pagebreak

$-U_k \cdot U_k^T \cdot g_k$
\pagebreak

$U_k$
\pagebreak

$A_{ij}$
\pagebreak

$B_{ij}$
\pagebreak

\[ B_{ij} = \frac{3}{2} \left(\frac{1}{4 \pi \varepsilon_0}\right)^\frac{1}{2} \frac{e \hbar \sqrt{m_e} \alpha_i \alpha_j}{\sqrt{\frac{\alpha_i}{N_i} + \sqrt{\frac{\alpha_j}{N_j}}}} \]
\pagebreak

\[ A_{ij} = \frac{1}2{} B_{ij} (R_i + R_j)^6 \]
\pagebreak

\[ S(\delta) = \sum_{i} \frac{h_i}{w_i (\delta_i-\delta)^2} \]
\pagebreak

$\delta$
\pagebreak

$\delta_i$
\pagebreak

$h_i$
\pagebreak

$w_i$
\pagebreak

$ \sqrt{k(x_*,x_*)-\sum_{i=1}^n \sum_{j=1}^n k(x_*,x_i)*k(x_*,x_j)-L_{ij} } $
\pagebreak

$ \sum_{i=1}^m (input_{ai} * input_{bi})^p $
\pagebreak

$ g(\sum_{i=1}^m f(input_{ai}, input_{bi})) $
\pagebreak

$ \sum_{i=1}^m (m1_{ai} * m2_{bi})^p $
\pagebreak

$ g(\sum_{i=1}^m f(m1_{ai}, m2_{bi})) $
\pagebreak

$ dist(a,b)= g(\sum_{i=1}^m f(x1,x2)) $
\pagebreak

$ \sum_{i=1}^m w_i * (input_{ai}- input_{bi})^2 $
\pagebreak

$ \sum_{i=1}^m w_i * (m1_{ai}- m2_{bi})^2 $
\pagebreak

$ sqrt(\sum_i (row1_i-row2_i)^2) $
\pagebreak

$ sqrt(\sum_i cv_i^2) $
\pagebreak

$ sqrt(\sum_i (cv1_i-cv2_i)^2) $
\pagebreak

$ cv^T*cv = \sum_i cv_i^2 $
\pagebreak

$\varepsilon$
\pagebreak

$\bar{\kappa}$
\pagebreak

\[ \phi_{x,y,z} = \sum_i \frac{1}{4 \pi \varepsilon \varepsilon_0} \frac{q_i}{r} e^{-\frac{r}{d}} \]
\pagebreak

\[ \varepsilon_0 = \frac{1}{27} \left( \sum_{i=1}^{26} \varepsilon_i + \varepsilon_0 \right) \]
\pagebreak

\[ \varepsilon_0 = \frac{1}{\sum_{i=1}^{26} \frac{1}{\varepsilon_i} + \frac{1}{\varepsilon_0}} \]
\pagebreak

$\mathrm{J}\cdot\mathrm{mol}^{-1}\cdot A^{-2}$
\pagebreak

$C$
\pagebreak

$\gamma A$
\pagebreak

$\mathrm{J}\cdot\mathrm{mol}^{-1}$
\pagebreak

$5.41 \mathrm{cal}\cdot\mathrm{mol}^{-1}\cdot A^{-2} = 22.635 \mathrm{J}\cdot\mathrm{mol}^{-1}\cdot A^{-2}$
\pagebreak

$6 \mathrm{cal}\cdot\mathrm{mol}^{-1}\cdot A^{-2} = 25.1 \mathrm{J}\cdot\mathrm{mol}^{-1}\cdot A^{-2}$
\pagebreak

$0.921 \mathrm{kcal}\cdot\mathrm{mol}^{-1} = 3.855 \mathrm{kJ}\cdot\mathrm{mol}^{-1}$
\pagebreak

$\AA^2$
\pagebreak

$\AA^3$
\pagebreak

$\chi_1$
\pagebreak

$\chi_2$
\pagebreak

$\chi_3$
\pagebreak

$\chi_4$
\pagebreak

\end{document}
